Fixing Nat

Nat.v
@@ -18,10 +18,10 @@ Fixpoint nat_rec_ (p : Obj)
   (HS : forall (p0 : Obj) (α : p ≤ p0),
        (forall (p : Obj) (α0 : p0 ≤ p), P p (α ∘ α0) p #) ->
        P p0 (fun (R : Obj) (k : Hom p0 R) => α R k) p0 #)
-  (n : ᶠnat p):
+  (n : natᶠ p):
    P p # p # := match n with
-            | ᶠO _ =>    H0 p #
-            | ᶠS _ n0 => HS p #
+            | Oᶠ _ =>    H0 p #
+            | Sᶠ _ n0 => HS p #
                    (fun (p1 : Obj) (α1 : p ≤ p1) =>
                       nat_rec_ p1
                         (fun p1 f1 => P  p1 (α1 ∘ f1))
@@ -45,10 +45,10 @@ Forcing Translate foo using Obj Hom.
 Forcing Translate bar using Obj Hom.
 Forcing Translate qux using Obj Hom.
 
-Eval compute in ᶠbar.
-Eval compute in ᶠqux.
+Eval compute in barᶠ.
+Eval compute in quxᶠ.
 
-Check (eq_refl : ᶠbar = ᶠqux).
+Check (eq_refl : barᶠ = quxᶠ).
 
 Definition nat_mem : forall R, nat -> (nat -> R) -> R :=
   fun R : Type =>
@@ -63,67 +63,67 @@ Forcing Definition nat_rect : forall (P : nat -> Type),
     forall n : nat, nat_mem _ n P using Obj Hom.
 Proof.
 
-  intros p P H0 HS n. unfold ᶠnat_mem, ᶠnat_rec . set (n0 := n p #). clearbody n0; clear n.
+  intros p P H0 HS n. unfold nat_memᶠ, nat_recᶠ . set (n0 := n p #). clearbody n0; clear n.
 
   (* avoiding noise in the actual definition *)
   (* may be improved using LTac ? *)
   
   set (Type_of_P := fun p => forall p0 : Obj,
       p ≤ p0 ->
-      (forall p : Obj, p0 ≤ p -> ᶠnat p) ->
+      (forall p : Obj, p0 ≤ p -> natᶠ p) ->
       forall p : Obj, p0 ≤ p -> Type).
   set (Type_of_H0 := fun p (P:Type_of_P p) => forall (p0 : Obj) (α : p ≤ p0),
-       P p0 (# ∘ (α ∘ #)) (fun (p : Obj) (_ : p0 ≤ p) => ᶠO p) p0 #).
+       P p0 (# ∘ (α ∘ #)) (fun (p : Obj) (_ : p0 ≤ p) => Oᶠ p) p0 #).
   set (Type_of_HS := fun p (P:Type_of_P p) => forall (p0 : Obj) (α : p ≤ p0)
-         (n : forall p : Obj, p0 ≤ p -> ᶠnat p),
+         (n : forall p : Obj, p0 ≤ p -> natᶠ p),
        (forall (p1 : Obj) (α0 : p0 ≤ p1),
-        ᶠnat_mem p1
+        nat_memᶠ p1
           (fun (p : Obj) (_ : p1 ≤ p) (p2 : Obj) (_ : p ≤ p2) =>
            forall p3 : Obj, p2 ≤ p3 -> Type)
           (fun (p : Obj) (α1 : p1 ≤ p) => n p (# ∘ (α0 ∘ (α1 ∘ #))))
           (fun (p2 : Obj) (α1 : p1 ≤ p2) =>
            P p2 (# ∘ (# ∘ (α ∘ (# ∘ (# ∘ (α0 ∘ (α1 ∘ #)))))))) p1 
           #) ->
-       ᶠnat_mem p0
+       nat_memᶠ p0
          (fun (p : Obj) (_ : p0 ≤ p) (p1 : Obj) (_ : p ≤ p1) =>
           forall p2 : Obj, p1 ≤ p2 -> Type)
          (fun (p : Obj) (α0 : p0 ≤ p) =>
-          ᶠS p
+          Sᶠ p
             (fun (p1 : Obj) (α1 : p ≤ p1) => n p1 (# ∘ (α0 ∘ (α1 ∘ #)))))
          (fun (p1 : Obj) (α0 : p0 ≤ p1) =>
           P p1 (# ∘ (# ∘ (α ∘ (# ∘ (# ∘ (α0 ∘ #))))))) p0 
          #).
-  set (Type_of_Goal := fun p (P:Type_of_P p) (H0:Type_of_H0 p P) (HS:Type_of_HS p P) (n0: ᶠnat p) => nat_rec_ p
+  set (Type_of_Goal := fun p (P:Type_of_P p) (H0:Type_of_H0 p P) (HS:Type_of_HS p P) (n0: natᶠ p) => nat_rec_ p
      (fun (p0 : Obj) (_ : p ≤ p0) (p1 : Obj) (_ : p0 ≤ p1) =>
       (forall p2 : Obj,
        p1 ≤ p2 ->
-       (forall p3 : Obj, p2 ≤ p3 -> ᶠnat p3) ->
+       (forall p3 : Obj, p2 ≤ p3 -> natᶠ p3) ->
        forall p3 : Obj, p2 ≤ p3 -> Type) ->
       forall p2 : Obj, p1 ≤ p2 -> Type)
      (fun (p0 : Obj) (_ : p ≤ p0)
         (f : forall p1 : Obj,
              p0 ≤ p1 ->
-             (forall p2 : Obj, p1 ≤ p2 -> ᶠnat p2) ->
+             (forall p2 : Obj, p1 ≤ p2 -> natᶠ p2) ->
              forall p2 : Obj, p1 ≤ p2 -> Type) =>
-      f p0 # (fun (p1 : Obj) (_ : p0 ≤ p1) => ᶠO p1))
+      f p0 # (fun (p1 : Obj) (_ : p0 ≤ p1) => Oᶠ p1))
      (fun (p0 : Obj) (_ : p ≤ p0)
         (H : forall p1 : Obj,
              p0 ≤ p1 ->
              (forall p2 : Obj,
               p1 ≤ p2 ->
-              (forall p3 : Obj, p2 ≤ p3 -> ᶠnat p3) ->
+              (forall p3 : Obj, p2 ≤ p3 -> natᶠ p3) ->
               forall p3 : Obj, p2 ≤ p3 -> Type) ->
              forall p2 : Obj, p1 ≤ p2 -> Type)
         (f : forall p1 : Obj,
              p0 ≤ p1 ->
-             (forall p2 : Obj, p1 ≤ p2 -> ᶠnat p2) ->
+             (forall p2 : Obj, p1 ≤ p2 -> natᶠ p2) ->
              forall p2 : Obj, p1 ≤ p2 -> Type) =>
       H p0 #
         (fun (p1 : Obj) (α0 : p0 ≤ p1)
-           (n : forall p2 : Obj, p1 ≤ p2 -> ᶠnat p2) =>
+           (n : forall p2 : Obj, p1 ≤ p2 -> natᶠ p2) =>
          f p1 (fun (R : Obj) (k : Hom p1 R) => α0 R k)
            (fun (p2 : Obj) (α1 : p1 ≤ p2) =>
-            ᶠS p2 (fun (p3 : Obj) (α2 : p2 ≤ p3) => n p3 (α1 ∘ α2))))) n0
+            Sᶠ p2 (fun (p3 : Obj) (α2 : p2 ≤ p3) => n p3 (α1 ∘ α2))))) n0
      (fun (p0 : Obj) (α : p ≤ p0) =>
       P p0 (fun (R : Obj) (k : Hom p0 R) => α R k)) p 
      #).
@@ -137,10 +137,10 @@ Proof.
               (P : Type_of_P p)
               (H0 : Type_of_H0 p P)
               (HS : Type_of_HS p P)
-              (n0 : ᶠnat p) : Type_of_Goal p P H0 HS n0
-             := match n0 as n1 in ᶠnat _ return Type_of_Goal p P H0 HS n1 with
-            | ᶠO _ =>   H0 p #
-            | ᶠS _ n => HS p # n
+              (n0 : natᶠ p) : Type_of_Goal p P H0 HS n0
+             := match n0 as n1 in natᶠ _ return Type_of_Goal p P H0 HS n1 with
+            | Oᶠ _ =>   H0 p #
+            | Sᶠ _ n => HS p # n
                    (fun (p1 : Obj) (α1 : p ≤ p1) =>
                       F p1
                         (fun p1 f1 => P  p1 (α1 ∘ f1))
@@ -162,10 +162,10 @@ Definition qux2 := fun (P : nat -> Type) (H0 : P O)
 Forcing Translate bar2 using Obj Hom.
 Forcing Translate qux2 using Obj Hom.
 
-Eval compute in ᶠbar2.
-Eval compute in ᶠqux2.
+Eval compute in bar2ᶠ.
+Eval compute in qux2ᶠ.
 
-Check (eq_refl : ᶠbar2 = ᶠqux2).
+Check (eq_refl : bar2ᶠ = qux2ᶠ).
 
 
 End Nat.
